midterm-project/exercises/host.i.dfy
@@ -16,13 +16,15 @@ module Host {
 
   // Define your Host protocol state machine here.
   datatype Constants = Constants(myId:HostId) {
-    predicate WF(id:HostId) { // host constants coupled to DistributedSystem Constants.
+    // host constants coupled to DistributedSystem Constants:
+    // DistributedSystem tells us our id so we can recognize inbound messages.
+    // TODO(jonh): get rid of ValidHosts; move hostCount in here instead.
+    predicate GroupWF(id:HostId) {
       myId == id
     }
   }
   datatype Variables = Variables(/* FILL ME IN! */)
 
-  // DistributedSystem tells us our id so we can recognize inbound messages.
   predicate Init(c:Constants, v:Variables) {
     true // Replace me
   }
